src/Assembly/Equivalence.v
@@ -1195,6 +1195,7 @@ Proof.
           | ident.prod_rect _ _ _
           | ident.bool_rect _
           | ident.bool_rect_nodep _
+          | ident.if_expect_true _
           | ident.nat_rect _
           | ident.eager_nat_rect _
           | ident.nat_rect_arrow _ _
