src/Language/APINotations.v
@@ -77,6 +77,7 @@ Module Compilers.
   Global Arguments ident_prod_rect {_ _ _} : assert.
   Global Arguments ident_bool_rect {_} : assert.
   Global Arguments ident_bool_rect_nodep {_} : assert.
+  Global Arguments ident_if_expect_true {_} : assert.
   Global Arguments ident_nat_rect {_} : assert.
   Global Arguments ident_nat_rect_arrow {_ _} : assert.
   Global Arguments ident_eager_nat_rect {_} : assert.
@@ -249,6 +250,7 @@ Module Compilers.
     Notation prod_rect := Compilers.ident_prod_rect (only parsing).
     Notation bool_rect := Compilers.ident_bool_rect (only parsing).
     Notation bool_rect_nodep := Compilers.ident_bool_rect_nodep (only parsing).
+    Notation if_expect_true := Compilers.ident_if_expect_true (only parsing).
     Notation nat_rect := Compilers.ident_nat_rect (only parsing).
     Notation nat_rect_arrow := Compilers.ident_nat_rect_arrow (only parsing).
     Notation eager_nat_rect := Compilers.ident_eager_nat_rect (only parsing).
